examples/dsls/mini_steel/tests/Pulse.Tests.fst
@@ -9,79 +9,6 @@ open Steel.FractionalPermission
 open FStar.Ghost
 #push-options "--print_universes --print_implicits"
 
-%splice_t[foo] (parse_and_check "return true")
-
-%splice_t[read] (parse_and_check "
-   fun (n:FStar.Ghost.erased u#0 Pulse.Steel.Wrapper.u32)
-       (r:Steel.ST.Reference.ref Pulse.Steel.Wrapper.u32)
-         requires (Steel.ST.Reference.pts_to #Pulse.Steel.Wrapper.u32 r Steel.FractionalPermission.full_perm (FStar.Ghost.reveal u#0 #Pulse.Steel.Wrapper.u32 n)) ->
-         Pulse.Steel.Wrapper.read n r
-   ")
-
-%splice_t[read2] (check (`(fun (n:erased u#0 u32) (r:ref u32) ->
-                              Pulse.Steel.Wrapper.read n r 
-                            <: stt u#0 u32
-                                (pts_to #u32 r full_perm (reveal u#0 #u32 n))
-                                (fun x -> pts_to #u32 r full_perm x))))
-
-%splice_t[read_alt_with_post] (parse_and_check "
-    fun (n:FStar.Ghost.erased u#0 Pulse.Steel.Wrapper.u32)
-        (r:Steel.ST.Reference.ref Pulse.Steel.Wrapper.u32)   
-          requires  (Steel.ST.Reference.pts_to #Pulse.Steel.Wrapper.u32 r Steel.FractionalPermission.full_perm (FStar.Ghost.reveal u#0 #Pulse.Steel.Wrapper.u32 n))
-          ensures _ . (Steel.ST.Reference.pts_to #Pulse.Steel.Wrapper.u32 r Steel.FractionalPermission.full_perm 
-                                                (FStar.Ghost.reveal u#0 #Pulse.Steel.Wrapper.u32 n)) ->
-          Pulse.Steel.Wrapper.read_alt n r
-    ")
-
- %splice_t[read_alt_with_post2] (parse_and_check "
-   fun (n:FStar.Ghost.erased u#0 Pulse.Steel.Wrapper.u32)
-       (r1:Steel.ST.Reference.ref Pulse.Steel.Wrapper.u32)
-       (r2:Steel.ST.Reference.ref Pulse.Steel.Wrapper.u32)
-         requires  (Steel.ST.Reference.pts_to #Pulse.Steel.Wrapper.u32 r1 Steel.FractionalPermission.full_perm (FStar.Ghost.reveal u#0 #Pulse.Steel.Wrapper.u32 n) *
-                    Steel.ST.Reference.pts_to #Pulse.Steel.Wrapper.u32 r2 Steel.FractionalPermission.full_perm (FStar.Ghost.reveal u#0 #Pulse.Steel.Wrapper.u32 n))
-         ensures _ . (Steel.ST.Reference.pts_to #Pulse.Steel.Wrapper.u32 r1 Steel.FractionalPermission.full_perm (FStar.Ghost.reveal u#0 #Pulse.Steel.Wrapper.u32 n) *
-                      Steel.ST.Reference.pts_to #Pulse.Steel.Wrapper.u32 r2 Steel.FractionalPermission.full_perm (FStar.Ghost.reveal u#0 #Pulse.Steel.Wrapper.u32 n)) ->
-         Pulse.Steel.Wrapper.read_alt n r2
-   ")
-
-%splice_t[read_refine] (parse_and_check "
-    fun (n:FStar.Ghost.erased u#0 Pulse.Steel.Wrapper.u32)
-        (r:Steel.ST.Reference.ref Pulse.Steel.Wrapper.u32)
-           requires (Steel.ST.Reference.pts_to #Pulse.Steel.Wrapper.u32 r Steel.FractionalPermission.full_perm (FStar.Ghost.reveal u#0 #Pulse.Steel.Wrapper.u32 n)) ->
-           Pulse.Steel.Wrapper.read_refine n r
-     ")
-
- %splice_t[write] (parse_and_check "
-    fun (n:FStar.Ghost.erased u#0 Pulse.Steel.Wrapper.u32)
-        (r1:Steel.ST.Reference.ref Pulse.Steel.Wrapper.u32)
-        (x:Pulse.Steel.Wrapper.u32)
-        (r2:Steel.ST.Reference.ref Pulse.Steel.Wrapper.u32)
-          requires (Steel.ST.Reference.pts_to #Pulse.Steel.Wrapper.u32 r1 Steel.FractionalPermission.full_perm (FStar.Ghost.reveal u#0 #Pulse.Steel.Wrapper.u32 n) *
-                    Steel.ST.Reference.pts_to #Pulse.Steel.Wrapper.u32 r2 Steel.FractionalPermission.full_perm (FStar.Ghost.reveal u#0 #Pulse.Steel.Wrapper.u32 n)) ->
-          Pulse.Steel.Wrapper.write n r2 x
-    ")
-
-//Bound variable escapes scope
-[@@ expect_failure]
- %splice_t[read_alt_write] (parse_and_check  "
-     fun (n:FStar.Ghost.erased u#0 Pulse.Steel.Wrapper.u32)
-         (r:Steel.ST.Reference.ref Pulse.Steel.Wrapper.u32)
-           requires (Steel.ST.Reference.pts_to #Pulse.Steel.Wrapper.u32 r Steel.FractionalPermission.full_perm 
-                                               (FStar.Ghost.reveal u#0 #Pulse.Steel.Wrapper.u32 n)) ->
-           let x = Pulse.Steel.Wrapper.read_alt n r;
-           Pulse.Steel.Wrapper.write n r x
-     ")
-
-
-%splice_t[read_alt_write_alt] (parse_and_check  "
-      fun (n:FStar.Ghost.erased u#0 Pulse.Steel.Wrapper.u32)
-          (r:Steel.ST.Reference.ref Pulse.Steel.Wrapper.u32)
-           requires (Steel.ST.Reference.pts_to #Pulse.Steel.Wrapper.u32 r Steel.FractionalPermission.full_perm 
-                                               (FStar.Ghost.reveal u#0 #Pulse.Steel.Wrapper.u32 n)) ->
-            let x = Pulse.Steel.Wrapper.read_alt n r;
-            Pulse.Steel.Wrapper.write_alt n r x
-      ")
-
 %splice_t[swap] (parse_and_check "
     fun (n1:FStar.Ghost.erased u#0 Pulse.Steel.Wrapper.u32)
         (n2:FStar.Ghost.erased u#0 Pulse.Steel.Wrapper.u32)
@@ -92,24 +19,8 @@ open FStar.Ghost
           ensures _.(Steel.ST.Reference.pts_to #Pulse.Steel.Wrapper.u32 r1 Steel.FractionalPermission.full_perm (FStar.Ghost.reveal u#0 #Pulse.Steel.Wrapper.u32 n2) *
                      Steel.ST.Reference.pts_to #Pulse.Steel.Wrapper.u32 r2 Steel.FractionalPermission.full_perm (FStar.Ghost.reveal u#0 #Pulse.Steel.Wrapper.u32 n1)) ->
 
-          let x = Pulse.Steel.Wrapper.read_refine n1 r1;
-          let y = Pulse.Steel.Wrapper.read_refine n2 r2;
-          Pulse.Steel.Wrapper.write n1 r1 y;
-          Pulse.Steel.Wrapper.write n2 r2 x
+          let x = Pulse.Steel.Wrapper.read_refine r1;
+          let y = Pulse.Steel.Wrapper.read_refine r2;
+          Pulse.Steel.Wrapper.write r1 y;
+          Pulse.Steel.Wrapper.write r2 x
     ")
-    
-//This one doesn't work yet ... some bug in translating the quoted term
-[@@expect_failure]
-%splice_t[swap2] (check (`(fun (n1 n2:erased u#0 u32)
-                             (r1 r2:ref u32) ->
-                        (let x = read_refine n1 r1 in
-                         let y = read_refine n2 r2 in
-                         write n1 r1 y;
-                         write n2 r2 x) <:
-                         stt u#0 unit 
-                          (pts_to #u32 r1 full_perm (reveal u#0 #u32 n1) `star` 
-                           pts_to #u32 r2 full_perm (reveal u#0 #u32 n2))
-                          (fun _ -> 
-                           pts_to #u32 r1 full_perm (reveal u#0 #u32 n2) `star` 
-                           pts_to #u32 r2 full_perm (reveal u#0 #u32 n1)))))
-    
